Splinter/Betree/BranchedBetree.i.dfy
@@ -1,0 +1,1087 @@
+// Copyright 2018-2021 VMware, Inc., Microsoft Inc., Carnegie Mellon University, ETH Zurich, and University of Washington
+// SPDX-License-Identifier: BSD-2-Clause
+
+// include "PivotBetree.i.dfy"
+include "LinkedBetree.i.dfy"
+include "../../lib/Buckets/BoundedPivotsLib.i.dfy"
+include "../Journal/GenericDisk.i.dfy"
+include "Domain.i.dfy"
+include "LinkedForest.i.dfy"
+include "SplitRequest.i.dfy"
+
+// TODO:
+// This module deals with 
+// 1. Concretize buffer implementation with Forest (seqs of B+ tree)
+// 2. Filter should be implicitly tracked by pivot table (no more apply filters)
+//    - In LinkedBetree we did not restrict the range of splitted child
+// 3. Track active buffers for each child, as we don't want to visit a buffer that is flushed to a child already
+
+module BranchedBetreeMod
+{
+  import opened BoundedPivotsLib
+  import opened DomainMod
+  import opened GenericDisk
+  import opened KeyType
+  import opened LSNMod
+  import opened MemtableMod
+  import opened MsgHistoryMod
+  import opened Options
+  import opened Sequences
+  import opened StampedMod
+  import opened Upperbounded_Lexicographic_Byte_Order_Impl
+  import opened Upperbounded_Lexicographic_Byte_Order_Impl.Ord
+  import opened ValueMessage
+  import opened Maps
+  import TotalKMMapMod
+  import opened SplitRequestMod
+
+  import LF = LinkedForestMod
+  import LB = LinkedBranchMod
+
+  type Pointer = GenericDisk.Pointer
+  type Address = GenericDisk.Address
+  type StampedBetree = Stamped<LinkedBetree>
+  type StampedForest = Stamped<LF.LinkedForest> // TODO: revisit
+
+  function EmptyLinkedBetree() : (out: LinkedBetree)
+  {
+    LinkedBetree(None, EmptyDisk())
+  }
+
+  function EmptyImage() : StampedBetree
+  {
+    Stamped(EmptyLinkedBetree(), 0)
+  }
+
+  type Element = Upperbounded_Lexicographic_Byte_Order_Impl.Ord.Element
+
+  datatype TransitionLabel =
+      QueryLabel(endLsn: LSN, key: Key, value: Value)
+    | PutLabel(puts: MsgHistory)
+    | QueryEndLsnLabel(endLsn: LSN)
+    | FreezeAsLabel(linkedBetree: StampedBetree, forest: StampedForest)
+     // Internal-x labels refine to no-ops at the abstract spec
+    | InternalAllocationsLabel(addrs: seq<Address>)  // for steps that involve allocating new pages
+    | InternalLabel()   // Local No-op label
+
+
+  datatype BetreeNode = BetreeNode(
+    // bundle's filter apply to multiple branches
+    buffers: seq<Address>, // Forest Disk
+    pivotTable: PivotTable,
+    children: seq<Pointer>, // Betree Disk
+    activeBufferRanges: seq<nat>  // parallel DS to children array, each entry stores the start of active buffer range for the corresponding child
+  ) {
+    predicate WF() {
+      && (BetreeNode? ==>
+        && WFPivots(pivotTable)
+        && |children| == NumBuckets(pivotTable)
+        && |children| == |activeBufferRanges|
+        && (forall i:nat | i < |activeBufferRanges| :: activeBufferRanges[i] <= |buffers|))
+    }
+
+    predicate ValidChildIndex(childIdx: nat)
+    {
+      && BetreeNode?
+      && childIdx < NumBuckets(pivotTable)
+    }
+
+    predicate OccupiedChildIndex(childIdx: nat)
+      requires WF()
+    {
+      && ValidChildIndex(childIdx)
+      && children[childIdx].Some?
+    }
+
+    function PushBufferStack(addr: Address) : (out: BetreeNode)
+      requires WF()
+      requires BetreeNode?
+      ensures out.WF()
+    {
+      BetreeNode(buffers + [addr], pivotTable, children, activeBufferRanges)
+    }
+
+    predicate IsLeaf()
+    {
+      && |children|==1
+      && children[0].None?
+    }
+
+    predicate IsIndex()
+    {
+      && (forall i | 0 <= i < |children| :: children[i].Some?)
+    }
+
+    function MyDomain() : (out: Domain)
+      requires WF()
+    {
+      Domain(pivotTable[0], Last(pivotTable))
+    }
+
+    function DomainRoutedToChild(childIdx: nat) : (out: Domain)
+      requires WF()
+      requires BetreeNode?
+      requires ValidChildIndex(childIdx)
+      ensures out.WF()
+    {
+      var out := Domain(pivotTable[childIdx], pivotTable[childIdx+1]);
+      reveal_IsStrictlySorted();
+      out.reveal_SaneKeys();
+      out
+    }
+
+    predicate KeyInDomain(key: Key)
+    {
+      && WF()
+      && BetreeNode?
+      && BoundedKey(pivotTable, key)
+    }
+
+    // // Redundant; should equal domain.KeySet() for the domain specified by the pivotTable.
+    // function KeySet() : iset<Key>
+    //   requires WF()
+    //   requires BetreeNode?  // TODO(jonh): trouble for Nils?
+    // {
+    //   iset key | KeyInDomain(key)
+    // }
+
+    function ChildPtr(key: Key) : Pointer
+      requires KeyInDomain(key)
+    {
+      children[Route(pivotTable, key)]
+    }
+    
+    function ChildBufferRange(key: Key) : (i: nat)
+      requires KeyInDomain(key)
+    {
+      activeBufferRanges[Route(pivotTable, key)]
+    }
+
+    // TODO(jonh): Again, Split has a bunch of duplicated (complex) definitions duplicated from PivotBetree.
+    // Would be nice to find a way to factor out the structure duplicated across layers without
+    // making the state machines difficult to read.
+
+    // Called on leaf; creates a new pivot
+    function SplitLeaf(splitKey: Key) : (out: (BetreeNode, BetreeNode))
+      requires WF()
+      requires IsLeaf()
+      requires MyDomain().Contains(splitKey)
+      requires splitKey != MyDomain().start.e
+      ensures out.0.WF() && out.1.WF()
+    {
+      var newLeft := BetreeNode(buffers, [pivotTable[0], Element(splitKey)], [None], [0]);
+      var newRight := BetreeNode(buffers, [Element(splitKey), pivotTable[1]], [None], [0]);
+      assert newLeft.WF() by { Keyspace.reveal_IsStrictlySorted(); }
+      assert newRight.WF() by { Keyspace.reveal_IsStrictlySorted(); }
+      (newLeft, newRight)
+    }
+
+    // Called on index; lifts an existing pivot from the child
+    function SplitIndex(pivotIdx: nat) : (out: (BetreeNode, BetreeNode))
+      requires WF()
+      requires IsIndex()
+      requires 0 < pivotIdx < |pivotTable|-1
+      ensures out.0.WF() && out.1.WF()
+    {
+      var splitElt := pivotTable[pivotIdx];
+      var leftFilter := Domain(MyDomain().start, splitElt);
+      var rightFilter := Domain(splitElt, MyDomain().end);
+
+      var newLeft := BetreeNode(buffers, pivotTable[..pivotIdx+1], children[..pivotIdx], activeBufferRanges[..pivotIdx]);
+      var newRight := BetreeNode(buffers, pivotTable[pivotIdx..], children[pivotIdx..], activeBufferRanges[pivotIdx..]);
+      WFSlice(pivotTable, 0, pivotIdx+1);
+      WFSuffix(pivotTable, pivotIdx);
+      //assert WFChildren(children);  // trigger TODO(jonh) delete
+      assert newLeft.WF();
+      assert newRight.WF();
+      (newLeft, newRight)
+    }
+  }
+
+  // PivotTable constructor for a total domain
+  function TotalPivotTable() : PivotTable
+  {
+    [TotalDomain().start, TotalDomain().end]
+  }
+
+  // BetreeNode constructor for empty node
+  function EmptyRoot(domain: Domain) : (out: BetreeNode)
+    requires domain.WF()
+    requires domain.Domain?
+    ensures out.WF()
+  {
+    var pivotTable := [domain.start, domain.end];
+    domain.reveal_SaneKeys();  /* jonh suspicious lt leak */
+    assert Keyspace.IsStrictlySorted(pivotTable) by { reveal_IsStrictlySorted(); }  /* jonh suspicious lt leak */
+    BetreeNode([], pivotTable, [None], [0])
+  }
+
+  datatype DiskView = DiskView(entries: map<Address, BetreeNode>)
+  {
+    // TODO(jonh): some duplication with LinkedJournal.DiskView; refactor into library superclassish thing?
+    // Or a generic with GenericDisk.DiskView<T>?
+    // BetreeNodes are WF()
+    predicate EntriesWF()
+    {
+      (forall addr | addr in entries :: entries[addr].WF())
+    }
+
+    predicate IsNondanglingPointer(ptr: Pointer)
+    {
+      && ptr.Some? ==> ptr.value in entries
+    }
+
+    predicate NodeHasNondanglingChildPtrs(node: BetreeNode)
+      requires EntriesWF()
+      requires node.WF()
+    {
+      node.BetreeNode? ==> (
+        && (forall idx:nat | node.ValidChildIndex(idx) :: IsNondanglingPointer(node.children[idx]))
+      )
+    }
+
+    predicate ChildLinked(node: BetreeNode, idx: nat)
+      requires EntriesWF()
+      requires node.WF()
+      requires NodeHasNondanglingChildPtrs(node)
+      requires node.BetreeNode?
+      requires node.ValidChildIndex(idx)
+    {
+      node.children[idx].Some? ==> (
+        entries[node.children[idx].value].MyDomain() == node.DomainRoutedToChild(idx)
+      )
+    }
+
+    predicate NodeHasLinkedChildren(node: BetreeNode)
+      requires EntriesWF()
+      requires node.WF()
+      requires NodeHasNondanglingChildPtrs(node)
+    {
+      node.BetreeNode? ==> (
+        && (forall idx | node.ValidChildIndex(idx) :: ChildLinked(node, idx))
+      )
+    }
+
+    predicate HealthyChildPointers()  // i.e. disk is closed wrt to all the pointers in the nodes on disk
+      requires EntriesWF()
+    {
+      && (forall addr | addr in entries :: NodeHasNondanglingChildPtrs(entries[addr]))
+      && (forall addr | addr in entries :: NodeHasLinkedChildren(entries[addr]))
+    }
+
+    predicate WF()
+    {
+      && EntriesWF()
+      && HealthyChildPointers()
+    }
+
+    function Get(ptr: Pointer) : BetreeNode
+      // requires WF()
+      requires IsNondanglingPointer(ptr)
+      requires ptr.Some?
+    {
+      entries[ptr.value]
+    }
+
+    // buffer not in entries, it belongs to a different disk
+    predicate BufferInNode(buffer: Address)
+    {
+      (exists addr :: addr in entries && entries[addr].BetreeNode? && buffer in entries[addr].buffers)
+    }
+
+    function Buffers() : iset<Address>
+    {
+      iset buffer:Address | BufferInNode(buffer)
+    }
+
+    predicate AgreesWithDisk(other: DiskView)
+    {
+      MapsAgree(entries, other.entries)
+    }
+
+    predicate IsSubsetOf(other: DiskView)
+    {
+      && entries.Keys <= other.entries.Keys
+      && AgreesWithDisk(other)
+    }
+
+    // The node at this address has child pointers that respect ranking
+    predicate NodeChildrenRespectsRank(ranking: Ranking, addr: Address)
+      requires WF()
+      requires addr in entries
+      requires addr in ranking
+    {
+      && var node := entries[addr];
+      && (forall childIdx:nat | node.ValidChildIndex(childIdx) && node.children[childIdx].Some? ::
+        && node.children[childIdx].value in ranking  // ranking is closed
+        && ranking[node.children[childIdx].value] < ranking[addr]  // decreases
+      )
+    }
+
+    // Together with NodeChildrenRespectsRank, this says that ranking is closed
+    predicate ValidRanking(ranking: Ranking)
+      requires WF()
+    {
+      forall addr |
+        && addr in ranking
+        && addr in entries
+      ::
+        NodeChildrenRespectsRank(ranking, addr)
+    }
+
+    predicate IsFresh(addrs: set<Address>) {
+      addrs !! entries.Keys
+    }
+
+    // returns a new diskview with the new entry inserted
+    function ModifyDisk(addr: Address, item: BetreeNode) : DiskView{
+      DiskView.DiskView(entries[addr := item])
+    }
+  }
+
+  function EmptyDisk() : DiskView {
+    DiskView.DiskView(map[])
+  }
+
+  // This is the unit of interpretation: A LinkedBetree has enough info in it to interpret to a PivotBetree.BetreeNode.
+  datatype LinkedBetree = LinkedBetree(
+    root: Pointer,
+    diskView: DiskView
+  )
+  {
+    predicate WF() {
+      && diskView.WF()
+      && diskView.IsNondanglingPointer(root)
+    }
+
+    predicate HasRoot() {
+      && diskView.IsNondanglingPointer(root)
+      && root.Some?
+    }
+
+    function Root() : BetreeNode
+      requires HasRoot()
+    {
+      diskView.Get(root)
+    }
+
+    function ChildAtIdx(idx: nat) : LinkedBetree
+      requires WF()
+      requires HasRoot()
+      requires Root().ValidChildIndex(idx)
+    {
+      LinkedBetree(Root().children[idx], diskView)
+    }
+
+    function ChildForKey(key: Key) : LinkedBetree
+      requires HasRoot()
+      requires Root().KeyInDomain(key)
+    {
+      LinkedBetree(Root().ChildPtr(key), diskView)
+    }
+
+    function GetRank(ranking: Ranking) : nat
+      requires WF()
+    {
+      if HasRoot() && root.value in ranking then ranking[root.value]+1 else 0
+    }
+
+    function GetChildCount() : nat
+      requires WF()
+    {
+      if HasRoot() then |Root().children| else 0
+    }
+
+    // this says that ranking is closed
+    predicate ValidRanking(ranking: Ranking)
+      requires WF()
+    {
+      && diskView.ValidRanking(ranking)
+      && (HasRoot() ==> root.value in ranking)  // ranking covers tree from this root
+    }
+
+    predicate Acyclic()
+    {
+      && WF()
+      && (exists ranking :: ValidRanking(ranking))
+    }
+
+    function TheRanking() : Ranking
+      requires Acyclic()
+    {
+      var out :| ValidRanking(out);
+      out
+    }
+
+    function BuildTightTree() : (out: LinkedBetree)
+      ensures out.diskView.IsSubsetOf(diskView)
+    {
+      if ! Acyclic() then
+        // Need this case because at the state machine I don't have proof that after an
+        // operation, that the new state is acyclic
+        this
+      else
+        var tightDv := DiskView.DiskView(MapRestrict(diskView.entries, ReachableAddrs()));
+        LinkedBetree(root, tightDv)
+    }
+
+    function ReachableAddrs() : set<Address>
+      requires Acyclic()
+    {
+      ReachableAddrsUsingRanking(TheRanking())
+    }
+
+    function ReachableAddrsUsingRanking(ranking: Ranking) : (out: set<Address>)
+      requires WF()
+      requires ValidRanking(ranking)
+      ensures HasRoot() ==> root.value in out
+      ensures out <= diskView.entries.Keys
+      decreases GetRank(ranking)
+    {
+      if !HasRoot() then {}
+      else
+        var numChildren := |Root().children|;
+        var subTreeAddrs := seq(numChildren, i requires 0 <= i < numChildren => ChildAtIdx(i).ReachableAddrsUsingRanking(ranking));
+        Sets.UnionSeqOfSetsSoundness(subTreeAddrs);
+        {root.value} + Sets.UnionSeqOfSets(subTreeAddrs)
+    }
+    
+    predicate CanSplitParent(request: SplitRequest)
+    {
+      && WF()
+      && HasRoot()
+      && Root().ValidChildIndex(request.childIdx)
+      && var child := ChildAtIdx(request.childIdx);
+      && child.HasRoot()
+      && match request {
+        case SplitLeaf(_, splitKey) => child.Root().SplitLeaf.requires(splitKey)
+        case SplitIndex(_, childPivotIdx) => child.Root().SplitIndex.requires(childPivotIdx)
+      }
+    }
+
+    function SplitKey(request: SplitRequest) : (out: Key)
+      requires WF()
+      requires CanSplitParent(request)
+      ensures PivotInsertable(Root().pivotTable, request.childIdx+1, out)
+    {
+      var oldChild := ChildAtIdx(request.childIdx);
+      var out := if request.SplitLeaf? then request.splitKey else oldChild.Root().pivotTable[request.childPivotIdx].e;
+
+      assert PivotInsertable(Root().pivotTable, request.childIdx+1, out) by {
+        Keyspace.reveal_IsStrictlySorted();
+      }
+      WFPivotsInsert(Root().pivotTable, request.childIdx+1, out);
+
+      out
+    }
+
+    function SplitParent(request: SplitRequest, newAddrs: SplitAddrs) : (out: LinkedBetree)
+      requires WF()
+      requires CanSplitParent(request)
+    {
+      var oldChild := ChildAtIdx(request.childIdx);
+      var (newLeftChild, newRightChild) := if request.SplitLeaf? then oldChild.Root().SplitLeaf(request.splitKey) else oldChild.Root().SplitIndex(request.childPivotIdx);
+      var newChildren := replace1with2(Root().children, Some(newAddrs.left), Some(newAddrs.right), request.childIdx);
+      var childActiveRange := Root().activeBufferRanges[request.childIdx];
+      var newactiveBufferRanges := replace1with2(Root().activeBufferRanges, childActiveRange, childActiveRange, request.childIdx);
+
+      // new children replace 1with2 
+      var newParent := BetreeNode(Root().buffers, InsertPivot(Root().pivotTable, request.childIdx+1, SplitKey(request)), newChildren, newactiveBufferRanges);
+
+      var dv' := diskView.ModifyDisk(newAddrs.left, newLeftChild).ModifyDisk(newAddrs.right, newRightChild).ModifyDisk(newAddrs.parent, newParent);
+      LinkedBetree(Pointer.Some(newAddrs.parent), dv')
+    }
+
+    lemma SplitParentCanSubstitute(request: SplitRequest, newAddrs: SplitAddrs)
+      requires CanSplitParent(request)
+      requires newAddrs.HasUniqueElems()  // frameity frame frame
+      requires diskView.IsFresh(newAddrs.Repr())  // frameity frame frame
+      ensures SplitParent(request, newAddrs).WF()
+      ensures SplitParent(request, newAddrs).Root().MyDomain() == Root().MyDomain()
+    {
+      var dv := SplitParent(request, newAddrs).diskView;
+      var newParent := SplitParent(request, newAddrs).Root();
+
+      WFPivotsInsert(Root().pivotTable, request.childIdx+1, SplitKey(request));
+
+      forall idx:nat | newParent.ValidChildIndex(idx)
+      ensures dv.IsNondanglingPointer(newParent.children[idx]) {
+        if request.childIdx+1 < idx {
+          assert dv.IsNondanglingPointer(Root().children[idx-1]);  // seq offset trigger
+        }
+      }
+
+      forall idx:nat | newParent.ValidChildIndex(idx)
+      ensures dv.ChildLinked(newParent, idx) {
+        if idx < request.childIdx {
+          assert diskView.ChildLinked(Root(), idx);  // seq offset trigger
+        } else if request.childIdx+1 < idx {
+          assert diskView.ChildLinked(Root(), idx-1);  // seq offset trigger
+        }
+      }
+
+      forall i: nat | i < |newParent.activeBufferRanges|
+        ensures newParent.activeBufferRanges[i] <= |newParent.buffers|
+      {
+        if i > request.childIdx + 1 {
+          assert newParent.activeBufferRanges[i] == Root().activeBufferRanges[i-1];
+        }
+      }
+
+      if request.SplitIndex? {
+        var child := ChildAtIdx(request.childIdx).Root();
+        var left := dv.entries[newAddrs.left];
+        var right := dv.entries[newAddrs.right];
+
+        forall idx:nat | left.ValidChildIndex(idx) ensures dv.ChildLinked(left, idx) {
+          assert diskView.ChildLinked(child, idx);
+          assert dv.ChildLinked(left, idx);
+        }
+
+        forall idx:nat | right.ValidChildIndex(idx) ensures dv.ChildLinked(right, idx) {
+          assert diskView.ChildLinked(child, idx+request.childPivotIdx);
+          assert dv.ChildLinked(right, idx);
+        }
+      }
+      // assert dv.NodeHasLinkedChildren(dv.entries[newAddrs.parent]);
+    }
+  }
+
+  // disk addresses that are created during a split
+  datatype SplitAddrs = SplitAddrs(left: Address, right: Address, parent: Address)
+  {
+    predicate HasUniqueElems() {
+      && left!=right
+      && right!=parent
+      && parent!=left
+    }
+
+    function Repr() : set<Address> {
+      {left, right, parent}
+    }
+
+    function AsSeq() : seq<Address> {
+      [left, right, parent]
+    }
+  }
+
+  datatype Variables = Variables(
+    memtable: Memtable,
+    linked: LinkedBetree,
+    forestSM: LF.Variables)
+  {
+    predicate WF() {
+      && linked.WF()
+      && forestSM.WF()
+    }
+
+    predicate Valid() {
+      && DisjointForest()
+      && BoundedForest()
+    }
+
+    // linked diskView and forest diskView should have disjoint addresses
+    predicate DisjointForest() {
+      && linked.diskView.IsFresh(forestSM.Addresses())
+    }
+
+    // buffers in each node should be known to forest
+    predicate BoundedForest() {
+      && (forall addr, buffer | 
+        && addr in linked.diskView.entries 
+        && buffer in linked.diskView.entries[addr].buffers 
+        :: buffer in forestSM.forest.trees)
+    }
+  }
+
+  // TODO(jonh): SO much copypasta from PivotBetree! Library, paramaterize child mechanism?
+  datatype QueryReceiptLine = QueryReceiptLine(
+    linked: LinkedBetree,
+    result: Message)
+  {
+    predicate WF()
+    {
+      && result.Define?
+    }
+  }
+
+  datatype QueryReceipt = QueryReceipt(
+    key: Key,
+    linked: LinkedBetree,
+    forest: LF.LinkedForest,
+    lines: seq<QueryReceiptLine>)
+  {
+    predicate Structure()
+    {
+      && 0 < |lines|
+      && lines[0].linked == linked
+      && (forall i:nat | i < |lines| :: lines[i].linked.WF())
+      && (forall i:nat | i < |lines| :: lines[i].linked.root.Some? <==> i < |lines|-1)
+      && (forall i:nat | i < |lines| :: lines[i].linked.diskView == linked.diskView)
+      && Last(lines).result == Define(DefaultValue())
+      && linked.Acyclic()
+      && forest.WF() 
+    }
+
+    function Node(i: nat) : (out:BetreeNode)
+      requires Structure()
+      requires i < |lines| - 1  // last line is None ptr
+      ensures out.WF()
+    {
+      lines[i].linked.Root()
+    }
+
+    predicate AllLinesWF()
+    {
+      && Structure()
+      && (forall i:nat | i < |lines| :: lines[i].WF())
+      && (forall i:nat | i < |lines| :: lines[i].linked.Acyclic())
+      && (forall i:nat | i < |lines|-1 :: Node(i).KeyInDomain(key))
+      && (forall i:nat, buffer | i < |lines|-1 && buffer in Node(i).buffers :: forest.ValidTree(buffer))
+    }
+
+    predicate ChildLinkedAt(i: nat)
+      requires AllLinesWF()
+      requires i < |lines|-1
+    {
+      lines[i+1].linked.root == Node(i).ChildPtr(key)
+    }
+
+    function ResultAt(i: nat) : Message
+      requires i < |lines|
+    {
+      lines[i].result
+    }
+
+    predicate ResultLinkedAt(i: nat)
+      requires Structure()
+      requires AllLinesWF()
+      requires i < |lines| - 1
+    {
+      && var start := Node(i).ChildBufferRange(key); // only query on a child's active range
+      && var msg := forest.Query(key, Node(i).buffers[start..]);
+      && lines[i].result == Merge(msg, ResultAt(i+1))
+    }
+
+    predicate Valid()
+    {
+      && Structure()
+      && AllLinesWF()
+      && (forall i:nat | i < |lines| - 1 :: ChildLinkedAt(i))
+      && (forall i:nat | i < |lines| - 1 :: ResultLinkedAt(i))
+    }
+
+    predicate ValidFor(linked: LinkedBetree, forest: LF.LinkedForest, key: Key)
+    {
+      && Valid()
+      && this.linked == linked
+      && this.forest == forest
+      && this.key == key
+    }
+
+    function Result() : Message
+      requires Structure()
+    {
+      ResultAt(0)
+    }
+  }
+
+  predicate Query(v: Variables, v': Variables, lbl: TransitionLabel, receipt: QueryReceipt)
+  {
+    && lbl.QueryLabel?
+    && lbl.endLsn == v.memtable.seqEnd
+    && receipt.ValidFor(v.linked, v.forestSM.forest, lbl.key)
+    && Define(lbl.value) == Merge(v.memtable.Query(lbl.key), receipt.Result())
+    && v' == v
+  }
+
+  predicate Put(v: Variables, v': Variables, lbl: TransitionLabel)
+  {
+    && lbl.PutLabel?
+    && lbl.puts.WF()
+    && lbl.puts.seqStart == v.memtable.seqEnd
+    && v' == v.(
+        memtable := v.memtable.ApplyPuts(lbl.puts)
+      )
+  }
+
+  predicate QueryEndLsn(v: Variables, v': Variables, lbl: TransitionLabel)
+  {
+    && lbl.QueryEndLsnLabel?
+    && lbl.endLsn == v.memtable.seqEnd
+    && v' == v
+  }
+
+  predicate FreezeAs(v: Variables, v': Variables, lbl: TransitionLabel)
+  {
+    && lbl.FreezeAsLabel?
+    && v.WF()
+    && v.memtable.IsEmpty()
+    && lbl.linkedBetree == Stamped(v.linked, v.memtable.seqEnd)
+    && lbl.forest == Stamped(v.forestSM.forest, v.memtable.seqEnd)
+    && v' == v
+  }
+
+  type PathAddrs = seq<Address>
+
+  datatype Path = Path(linked: LinkedBetree, key: Key, depth: nat)
+  {
+    function Subpath() : (out: Path)
+      requires 0 < depth
+      requires linked.HasRoot()
+      requires linked.Root().KeyInDomain(key)
+    {
+      Path(linked.ChildForKey(key), key, depth-1)
+    }
+
+    predicate Valid()
+      decreases depth
+    {
+      && linked.Acyclic()
+      && linked.HasRoot()
+      && linked.Root().KeyInDomain(key)
+      && (0 < depth ==> linked.Root().IsIndex())
+      && (0 < depth ==> Subpath().Valid())  // implies path must lead to a non-nil node
+    }
+
+    function Target() : (out: LinkedBetree)
+      requires Valid()
+      ensures out.WF()
+      ensures out.root.Some?
+      ensures out.diskView == linked.diskView
+      ensures out.HasRoot() ==> out.root.value in out.diskView.entries
+      decreases depth
+    {
+      if 0 == depth
+      then linked
+      else Subpath().Target()
+    }
+
+    // Returns the address of all the nodes on the path, from root up to and including target
+    function AddrsOnPath() : set<Address> 
+      requires Valid()
+      decreases depth
+    {
+      if depth == 0 then {}
+      else Subpath().AddrsOnPath() + {linked.root.value}
+    }
+
+    predicate CanSubstitute(replacement: LinkedBetree, pathAddrs: PathAddrs)
+    {
+      && Valid()
+      && Target().HasRoot() // redundant with "path must lead to a non-nil node"?
+      && replacement.WF()
+      && replacement.HasRoot()
+      && replacement.Root().MyDomain() == Target().Root().MyDomain()
+      && depth == |pathAddrs|
+      && linked.diskView.IsSubsetOf(replacement.diskView)
+    }
+
+    lemma CanSubstituteSubpath(replacement: LinkedBetree, pathAddrs: PathAddrs)
+      requires CanSubstitute(replacement, pathAddrs)
+      requires 0 < depth
+      ensures Subpath().CanSubstitute(replacement, pathAddrs[1..])
+    {}
+
+    function Substitute(replacement: LinkedBetree, pathAddrs: PathAddrs) : (out: LinkedBetree)
+      requires CanSubstitute(replacement, pathAddrs)
+      decreases depth, 1
+    {
+      if depth == 0
+      then replacement
+      else
+        var node := linked.Root();
+        CanSubstituteSubpath(replacement, pathAddrs);
+        var subtree := Subpath().Substitute(replacement, pathAddrs[1..]);
+        var newChildren := node.children[Route(node.pivotTable, key) := subtree.root];
+        var newNode := BetreeNode(node.buffers, node.pivotTable, newChildren, node.activeBufferRanges);
+        var newDiskView := subtree.diskView.ModifyDisk(pathAddrs[0], newNode);
+        LinkedBetree(GenericDisk.Pointer.Some(pathAddrs[0]), newDiskView)
+    }
+  }
+
+  function InsertInternalFlushMemtableReplacement(oldRoot: LinkedBetree, memtableTree: Address, newRootAddr:Address) : (out: LinkedBetree)
+    requires oldRoot.WF()
+  {
+    var root' := 
+      if oldRoot.HasRoot()
+      then oldRoot.Root().PushBufferStack(memtableTree)
+      else BetreeNode([memtableTree], TotalPivotTable(), [None], [0]);
+
+    var dv' := oldRoot.diskView.ModifyDisk(newRootAddr, root');
+    LinkedBetree(Pointer.Some(newRootAddr), dv')
+  }
+
+  predicate InternalFlushMemtable(v: Variables, v': Variables, lbl: TransitionLabel, step: Step)
+  {
+    && v.WF()
+    && v.Valid()
+    && step.WF()
+    && lbl.InternalAllocationsLabel?
+    && step.InternalFlushMemtableStep?
+    && assert step.branch.I().WF() by { step.branch.WFI( step.branch.I() ); } // TODO: revisit
+    && step.branch.I().I() == v.memtable.buffer
+
+    && lbl.addrs == [step.newRootAddr] + step.branch.AddressesFromRoot() // TODO: revisit
+    // Subway Eat Fresh!
+    && v.linked.diskView.IsFresh({step.newRootAddr})
+    && v.linked.diskView.IsFresh(step.branch.diskView.Addresses())
+    && v.forestSM.forest.diskView.IsFresh({step.newRootAddr})
+    // && v.linked.diskView.IsFresh(step.branch.Addresses()) // captured in next step
+
+    && v'.linked == InsertInternalFlushMemtableReplacement(v.linked, step.branch.root, step.newRootAddr).BuildTightTree()
+    && v'.memtable == v.memtable.Drain()
+    && LF.Next(v.forestSM, v'.forestSM, LF.AddTreeLabel(step.branch))
+  }
+
+  function InsertGrowReplacement(oldRoot: LinkedBetree, newRootAddr:Address) : (out: LinkedBetree)
+    requires oldRoot.WF()
+  {
+    // The new root node
+    var root' := BetreeNode([], TotalPivotTable(), [oldRoot.root], [0]);
+    // The new diskview
+    var dv' := oldRoot.diskView.ModifyDisk(newRootAddr, root');
+    LinkedBetree(Pointer.Some(newRootAddr), dv')
+  }
+
+  predicate InternalGrow(v: Variables, v': Variables, lbl: TransitionLabel, step: Step)
+  {
+    && v.WF()
+    && step.WF()
+    && lbl.InternalAllocationsLabel?
+    && step.InternalGrowStep?
+    && lbl.addrs == [step.newRootAddr]
+    // Subway Eat Fresh!
+    && v.linked.diskView.IsFresh({step.newRootAddr})
+    && v'.linked == InsertGrowReplacement(v.linked, step.newRootAddr).BuildTightTree()
+    && v'.memtable == v.memtable  // UNCHANGED
+    && v'.forestSM == v.forestSM  // UNCHANGED
+  }
+
+//   predicate IsSplit(linked: LinkedBetree, linked': LinkedBetree, childIdx: nat, splitKey: Key)
+//   {
+//     && linked.WF()
+//     && linked'.WF()
+//     && linked.HasRoot()
+//     && linked'.HasRoot()
+//     && linked'.diskView.AgreesWithDisk(linked.diskView)
+//     && var root := linked.Root();
+//     && var root' := linked'.Root();
+
+//     && root.ValidChildIndex(childIdx)
+//     && PivotInsertable(root.pivotTable, childIdx, splitKey)
+//     && 0 < childIdx < NumBuckets(root.pivotTable) // Split can't extend domain of this node.
+//     && var oldChildPtr := root.children[childIdx];
+//     && oldChildPtr.Some?
+
+//     // Parent adds splitKey pivot; replaces child at childIdx with two children
+//     && root'.ValidChildIndex(childIdx+1)  // obvious once we have replace1with2, but we're not there yet
+//     && var leftChildPtr := root'.children[childIdx];
+//     && var rightChildPtr := root'.children[childIdx+1];
+//     && root' == root.(
+//       pivotTable := InsertPivot(root.pivotTable, childIdx, splitKey),
+
+//       // replace1with2 is just telling us about the structure of
+//       // root'.children: the prefix and suffix are identical, and the new left
+//       // & right child ptrs appear where childIdx once was. But it *doesn't*
+//       // say anything about the value of leftChildPtr (resp. rightChildPtr),
+//       // since we fetched those out of root'.children in the var statement
+//       // above. That's a "clever" trick to leave nondeterminism that says we
+//       // don't care what the actual values of those pointers are.
+//       children := replace1with2(root.children, leftChildPtr, rightChildPtr, childIdx)
+//       )
+
+//     // Children get correspending slices
+//     && leftChildPtr.Some?
+//     && rightChildPtr.Some?
+//     && var oldChild := linked.diskView.Get(oldChildPtr);
+//     && var leftChild := linked'.diskView.Get(leftChildPtr);
+//     && var rightChild := linked'.diskView.Get(rightChildPtr);
+//     && leftChild == oldChild.ApplyFilter(Domain(root.pivotTable[childIdx-1], Element(splitKey)))
+//     && rightChild == oldChild.ApplyFilter(Domain(Element(splitKey), root.pivotTable[childIdx]))
+
+//     // TODO(jonh): Say, ApplyFilter only affects buffers, but we also need to
+//     // carve up the pivot tables and children! ...in PivotBetree, too.
+//   }
+
+//   predicate InternalSplit(v: Variables, v': Variables, lbl: TransitionLabel, step: Step)
+//   {
+//     && v.WF()
+//     && lbl.InternalAllocationsLabel?
+//     && step.InternalSplitStep?
+//     && lbl.addrs == step.pathAddrs + step.newAddrs.AsSeq()
+//     && step.WF()
+//     && step.path.linked == v.linked
+//     && v.linked.diskView.IsFresh(step.newAddrs.Repr() + Set(step.pathAddrs))
+//     && step.path.Target().CanSplitParent(step.request)
+//     && var replacement := step.path.Target().SplitParent(step.request, step.newAddrs);
+//     && assert step.path.CanSubstitute(replacement, step.pathAddrs) by {
+//         step.path.Target().SplitParentCanSubstitute(step.request, step.newAddrs);
+//       } true
+//     && v'.linked == step.path.Substitute(replacement, step.pathAddrs).BuildTightTree()
+//     && v'.memtable == v.memtable  // UNCHANGED
+//   }
+
+//   function InsertFlushReplacement(target: LinkedBetree, childIdx:nat, targetAddr: Address, targetChildAddr: Address) : (out: LinkedBetree)
+//     requires target.WF()
+//     requires target.HasRoot()
+//     requires target.Root().OccupiedChildIndex(childIdx)
+//   {
+//     var root := target.Root();
+//     var keepKeys := AllKeys() - root.DomainRoutedToChild(childIdx).KeySet();
+//     var keptBuffers := root.buffers.ApplyFilter(keepKeys);
+//     var movedBuffers := root.buffers.ApplyFilter(root.DomainRoutedToChild(childIdx).KeySet());
+//     // BetreeNode of the new child, to be stored at targetChildAddr in the diskview
+//     var subroot := target.diskView.Get(root.children[childIdx]);
+//     var subroot' := BetreeNode(subroot.buffers.PushBufferStack(movedBuffers), subroot.pivotTable, subroot.children);
+
+//     // BetreeNode of the new root, to be stored at targetAddr in the diskview
+//     var children' := root.children[childIdx := Pointer.Some(targetChildAddr)];
+//     var root' := BetreeNode(keptBuffers, root.pivotTable, children');
+
+//     // The new diskview
+//     var dv' := target.diskView.ModifyDisk(targetAddr, root').ModifyDisk(targetChildAddr, subroot');
+//     LinkedBetree(Pointer.Some(targetAddr), dv')
+//   }
+
+//   predicate InternalFlush(v: Variables, v': Variables, lbl: TransitionLabel, step: Step)
+//   {
+//     && v.WF()
+//     && step.WF()
+//     && lbl.InternalAllocationsLabel?
+//     && step.InternalFlushStep?
+//     && lbl.addrs == step.pathAddrs + [step.targetAddr, step.targetChildAddr]
+//     && step.path.linked == v.linked
+//     && step.path.Valid()
+//     && step.path.Target().Root().OccupiedChildIndex(step.childIdx)  // the downstream child must exist
+//     && var replacement := InsertFlushReplacement(step.path.Target(), step.childIdx, step.targetAddr, step.targetChildAddr);
+//     && step.path.CanSubstitute(replacement, step.pathAddrs)
+//     // Subway Eat Fresh!
+//     && v.linked.diskView.IsFresh({step.targetAddr, step.targetChildAddr} + Set(step.pathAddrs))
+//     && v'.linked == step.path.Substitute(replacement, step.pathAddrs).BuildTightTree()
+//     && v'.memtable == v.memtable  // UNCHANGED
+//   }
+
+//   // target is the root node before it is compacted.
+//   // InsertReplacement returns a LinkedBetree that has the diskview of target with replacement placed at
+//   // the replacementAddr
+//   function InsertCompactReplacement(target: LinkedBetree, compactedBuffers: BufferStack, replacementAddr: Address) : (out: LinkedBetree)
+//     requires target.WF()
+//     requires target.HasRoot()
+//     requires target.Root().buffers.Equivalent(compactedBuffers)
+//     requires target.diskView.IsFresh({replacementAddr})
+//     ensures target.diskView.IsSubsetOf(out.diskView)
+//     ensures out.diskView.entries.Keys == target.diskView.entries.Keys + {replacementAddr}
+//     ensures out.WF()   // prereq to MyDomain()
+//     ensures out.HasRoot() && out.Root().MyDomain() == target.Root().MyDomain()
+//   {
+//     var root := target.Root();
+//     var newRoot := BetreeNode(compactedBuffers, root.pivotTable, root.children);
+//     var newDiskView := target.diskView.ModifyDisk(replacementAddr, newRoot);
+//     var out := LinkedBetree(GenericDisk.Pointer.Some(replacementAddr), newDiskView);
+//     out
+//   }
+
+//   predicate InternalCompact(v: Variables, v': Variables, lbl: TransitionLabel, step: Step)
+//   {
+//     && v.WF()
+//     && step.WF()
+//     && lbl.InternalAllocationsLabel?
+//     && step.InternalCompactStep?
+//     && lbl.addrs == step.pathAddrs + [step.targetAddr]
+//     && step.path.linked == v.linked
+//     && step.path.Valid()
+//     && step.path.Target().Root().buffers.Equivalent(step.compactedBuffers)
+//     // Subway Eat Fresh!
+//     && v.linked.diskView.IsFresh({step.targetAddr} + Set(step.pathAddrs))
+//     && v'.linked == step.path.Substitute(
+//         InsertCompactReplacement(step.path.Target(), step.compactedBuffers, step.targetAddr),
+//         step.pathAddrs
+//     ).BuildTightTree()
+//     && v'.memtable == v.memtable  // UNCHANGED
+//   }
+
+//   predicate InternalNoOp(v: Variables, v': Variables, lbl: TransitionLabel)
+//   {
+//     && lbl.InternalLabel?
+//     && v.WF()
+//     && v' == v
+//   }
+
+//   // public:
+
+//   predicate Init(v: Variables, stampedBetree: StampedBetree)
+//   {
+//     && v == Variables(EmptyMemtable(stampedBetree.seqEnd), stampedBetree.value)
+//   }
+
+  datatype Step =
+      QueryStep(receipt: QueryReceipt)
+    | PutStep()
+    | QueryEndLsnStep()
+    | FreezeAsStep()
+    // newRootAddr is the new address allocated for the new root
+    | InternalGrowStep(newRootAddr: Address)
+
+//     | InternalSplitStep(path: Path, request: SplitRequest, newAddrs: SplitAddrs, pathAddrs: PathAddrs)
+//       // request describes how the split applies (to an Index or Leaf); newAddrs are the new page addresses
+    | InternalFlushMemtableStep(newRootAddr: Address, branch: LB.LinkedBranch)
+//     | InternalFlushStep(path: Path, childIdx: nat, targetAddr: Address, targetChildAddr: Address, pathAddrs: PathAddrs)
+//       // targetAddr is the fresh address at which new node is placed, and targetChildAddr is for the new child receiving the flush
+//       // pathAddrs is the new addresses to place all its ancestors, used in substitution
+
+//     | InternalCompactStep(path: Path, compactedBuffers: BufferStack, targetAddr: Address, pathAddrs: PathAddrs)
+//       // targetAddr is the fresh address at which compactedNode is placed. pathAddrs is the new addresses to place all its ancestors
+//     | InternalNoOpStep()
+  {
+    predicate WF() {
+      match this {
+        case QueryStep(receipt) => receipt.Valid()
+        case InternalFlushMemtableStep(_, branch) => 
+          && branch.Acyclic()
+        // case InternalSplitStep(path, request, newAddrs, pathAddrs) =>
+//           && path.Valid()
+//           && path.depth == |pathAddrs|
+//           && SeqHasUniqueElems(pathAddrs)
+//           && path.Target().Root().ValidChildIndex(request.childIdx)
+//           && path.Target().CanSplitParent(request)
+//           && newAddrs.HasUniqueElems()
+//           && newAddrs.Repr() !! Set(pathAddrs)
+//         case InternalFlushStep(_, _, targetAddr, targetChildAddr, pathAddrs) =>
+//           && path.Valid()
+//           && path.Target().Root().ValidChildIndex(childIdx)
+//           && path.depth == |pathAddrs|
+//           && SeqHasUniqueElems(pathAddrs)
+//           && {targetAddr, targetChildAddr} !! Set(pathAddrs)
+//           && targetAddr != targetChildAddr
+//         case InternalCompactStep(path, compactedNode, targetAddr, pathAddrs) =>
+//           && path.Valid()
+//           && path.Target().Root().buffers.Equivalent(compactedBuffers)
+//           && path.depth == |pathAddrs|
+//           && SeqHasUniqueElems(pathAddrs)
+//           && {targetAddr} !! Set(pathAddrs)
+        case _ => true
+      }
+    }
+  }
+
+//   predicate NextStep(v: Variables, v': Variables, lbl: TransitionLabel, step: Step)
+//   {
+//     match step {
+//       case QueryStep(receipt) => Query(v, v', lbl, receipt)
+//       case PutStep() => Put(v, v', lbl)
+//       case QueryEndLsnStep() => QueryEndLsn(v, v', lbl)
+//       case FreezeAsStep() => FreezeAs(v, v', lbl)
+//       case InternalGrowStep(_) => InternalGrow(v, v', lbl, step)
+//       case InternalSplitStep(_, _, _, _) => InternalSplit(v, v', lbl, step)
+//       case InternalFlushMemtableStep(_) => InternalFlushMemtable(v, v', lbl, step)
+//       case InternalFlushStep(_, _, _, _, _) => InternalFlush(v, v', lbl, step)
+//       case InternalCompactStep(_, _, _, _) => InternalCompact(v, v', lbl, step)
+//       case InternalNoOpStep() => InternalNoOp(v, v', lbl)
+//     }
+//   }
+
+//   predicate Next(v: Variables, v': Variables, lbl: TransitionLabel) {
+//     exists step: Step :: NextStep(v, v', lbl, step)
+//   }
+}
